---
tags:
- math/algebra
- math/fundamentals
complete: true
index: null
---
### Summary
Basic Rules
$$
\begin{align*}
\text{Addition rule :}& \qquad x^n \cdot x^m = x^{n+m} \\
\\
\text{Subtraction rule :}& \qquad x^n \div x^m = x^{n-m} \\
\\
\text{Power rule :}& \qquad (x^n)^m = x^{n \cdot m} \\
\\
\text{Negative rule :}& \qquad x^{-n} = \frac{1}{x^{n}} \\
\\
\text{Fraction rule :}& \qquad x^\frac{m}{n} = \sqrt[n]{x^m} \\
\\
\text{Different \ base \ rule :}& \qquad x^n \cdot y^n = (x \cdot y)^n \\
\end{align*}
$$

Derived Formulas
$$
\begin{align*}
x^0 & = 1 \\
x^{-1} & = \frac{1}{x} \\
x^\frac{1}{2} & = \sqrt{x}
\end{align*}
$$

For [binomial theorem](/labyrinth/notes/math/ma1301/binomial_theorem), when extracting a constant ^e0fdcf
$$
\begin{align*}
(kx)^n & = k^n(x)^n \quad \text{(Different base rule)} \\
\\
ie. \ (4-x)^\frac{1}{2} &: \\
\\
(4-x)^\frac{1}{2} & = \left(4 \left(1-\frac{x}{4}\right)\right)^\frac{1}{2} \\
& = 4^\frac{1}{2} \left(1-\frac{x}{4}\right)^\frac{1}{2} = 2 \left(1-\frac{x}{4}\right)^\frac{1}{2}
\end{align*}
$$