---
tags:
- ma1301/chapter1
- math/calculus
complete: true
index: null
---
[Next](/labyrinth/notes/math/ma1301/geometric_series)

### Summary
Basic formulae
$$
\begin{align*}
nth \ term \ in \ a \ sequence &: \qquad a_{n} = a_{1}+(n-1)d \\
\\
Sum \ of \ first \ n \ terms \ in \ a \ series &: \qquad S_{n} = \frac{n}{2}(a_{1}+a_{n})=\frac{n}{2}(2a_{1}+(n-1)d) 
\end{align*}
$$

Derived formulae
$$
\begin{align*}
a_{1} & = S_{1} \\
\\
a_{n} & = S_{n}-S_{n-1}, \ for \ n \geq 2 \\
\\
n & = \frac{a_{n}-a_{1}}{d} + 1
\end{align*}
$$

[Summation](/labyrinth/notes/math/math_fundementals/summation_notation) notation
$$
\begin{align*}
\sum^n_{r=m} u_{r} , & \ where \ a_{r} \ has \ the \ form, \ r \cdot d \\
\\
No. \ of \ terms & = n-m+1
\end{align*}
$$

### Concept
Arithmetic sequence
$$
\begin{align*}
\lbrace a_{r} \rbrace^{n}_{r=1}: \quad a_{1}, \ & a_{2}, \ a_{3}, \ \dots \ , \ a_{n} \\
\\
such \ that: \quad a_{2} & = a_{1} + d \\
\\
a_{3} & = a_{2} + d = a_{1} + 2d
\end{align*}
$$

Proving arithmetic progression
$$
\begin{align*}
a_{n}-a_{n-1} & =a_{n+1}-a_{n}=d \\
\\
ie. & \ 1, \ 3, \ 5: \\
\\
a_{2}-a_{1} & =3-1 = 2\\
a_{3}-a_{2} & = 5-3 = 2 \\
d & =2, \ \therefore arithmetic \ sequence
\end{align*}
$$